BloodFilter.py
@@ -1,53 +1,42 @@
 from Blood import *
 
 
-# this class should be deprecated
-class BloodFilter():
-    def __init__(self):
-        raise DeprecationWarning("shouldn't be using this class")
-        self.conditions = []
-        self._filters = []
-
-    # add a conjunctive condition
-    # condition is a function that takes blood as argument
-    # and returns True or False to indicate whether this bag 
-    # of blood satisfies this condition.
-    def add_condition(self, condition):
-        self.conditions.append(condition)
-
-    # check if blood satisfies all conditions
-    def _check(self, blood: Blood) -> bool:
-        for c in self.conditions:
-            if not c(blood):
-                return False
-        return True
-
-    def filter(self, bloods: list) -> list:
-        res = []
-        for blood in bloods:
-            if self._check(blood):
-                res.append(blood)
-        return res
-
-
-
-# class BloodToSendFilter(BloodFilter):
-#     def __init__(self, blood_type: str = None):
-#         self.__init__2()
-#         if blood_type is not None:
-#             self.add_condition(lambda blood: blood.type == blood_type)
-
-#     def __init__2(self):
-#         super().__init__()
-#         self.add_condition(lambda blood: not blood.is_expired())
-#         self.add_condition(lambda blood: blood.is_good_blood())
-#         self.add_condition(lambda blood: blood.state == BloodState.IN_INVENTORY)
-
-
-# I wrote these functions so that they are easy to verify using dafny
-
+# in-place sort
 def sort_blood_by_useby_asc(bloods: list):
-    pass
+    sorted_tail: int = 0
+    while sorted_tail < len(bloods):
+        to_swap: int = sorted_tail
+        while to_swap >= 1 and bloods[to_swap - 1].use_by > bloods[to_swap].use_by:
+            bloods[to_swap - 1], bloods[to_swap] = bloods[to_swap], bloods[to_swap - 1]
+            to_swap -= 1
+        sorted_tail += 1
+
+def sort_blood_by_useby_desc(bloods: list):
+    sorted_tail: int = 0
+    while sorted_tail < len(bloods):
+        to_swap: int = sorted_tail
+        while to_swap >= 1 and bloods[to_swap - 1].use_by < bloods[to_swap].use_by:
+            bloods[to_swap - 1], bloods[to_swap] = bloods[to_swap], bloods[to_swap - 1]
+            to_swap -= 1
+        sorted_tail += 1
+
+def sort_blood_by_addtime_asc(bloods: list):
+    sorted_tail: int = 0
+    while sorted_tail < len(bloods):
+        to_swap: int = sorted_tail
+        while to_swap >= 1 and bloods[to_swap - 1].add_time > bloods[to_swap].add_time:
+            bloods[to_swap - 1], bloods[to_swap] = bloods[to_swap], bloods[to_swap - 1]
+            to_swap -= 1
+        sorted_tail += 1
+
+def sort_blood_by_addtime_desc(bloods: list):
+    sorted_tail: int = 0
+    while sorted_tail < len(bloods):
+        to_swap: int = sorted_tail
+        while to_swap >= 1 and bloods[to_swap - 1].add_time < bloods[to_swap].add_time:
+            bloods[to_swap - 1], bloods[to_swap] = bloods[to_swap], bloods[to_swap - 1]
+            to_swap -= 1
+        sorted_tail += 1
 
 def filter_blood_by_type(bloods: list, blood_type: str) -> list:
     res = []
