dafny/Blood.dfy
@@ -13,46 +13,23 @@ state:
 
 class Blood {
     var add_time: int;
-    var use_by: int; // UTC seconds since 1970-01-01 00:00:00 GTM
+    var use_by: int; // UTC seconds since 1970-01-01 00:00:00 GTM, could be negative
     var state: int;
     var test_state: int;
     var blood_type: string;
 
+    // just ensures the state is valid
     predicate valid()
     reads this
     {
-        add_time >= 0 && use_by >= 0 && state >= 1 && state <= 4
-    &&  test_state >=1 && test_state <= 3 && blood_type != ""
+        state >= 1 && state <= 4 && test_state >=1 && test_state <= 3
     }
 
     constructor(){
-
+        // sets the default state
+        state := 1;  // in inventory
+        test_state := 1;   // not tested
     }    
-
-    // constructor(add_time:int , use_by:int,state : int , test_state:int , blood_type:string) 
-    // modifies this;
-    // {
-    //     this.add_time := add_time;
-    //     this.use_by := use_by;
-    //     this.state := state;
-    //     this.test_state := test_state;
-    //     this.blood_type := blood_type;
-    // }
-
-    // should be moved to some upper level methods
-    method is_expired(curr_time: int) returns (expired: bool)
-    // requires curr_time is correct, but we cannot prove this
-    requires valid();
-    ensures valid();
-    ensures expired <==> use_by >= curr_time;
-    {
-        if (curr_time > use_by){
-            expired := false;
-        }
-        else {
-            expired := true;
-        }
-    }
 
     method blood_test(test_state:int) 
     requires test_state>=1 && test_state<=3;
